vGpd: formulate coh-2 for layers and use it to prove coh-2 for frames

theories/νSet/νGpd.v
@@ -636,6 +636,109 @@ Proof.
     now exact (mkCohPainting extraDepsCohs2).
 Defined.
 
+Definition mkCoh2FrameEndpointType {p k}
+  (depsCohs2: DepsCohs2 p.+1 k)
+  (extraDepsCohs2: DepsCohs2Extension p.+1 k depsCohs2)
+  (coh2Frames: mkCoh2FrameTypes (mkCohPaintings (depsCohs2; extraDepsCohs2)))
+  q (Hq: q <= k) r (Hr: r <= q) s (Hs: s <= r) (ε ω θ: arity)
+  (d: mkFrame (mkDepsRestr (depsCohs :=
+    toDepsCohs (mkCohFrames _ coh2Frames.1).1)).(1)): Type :=
+  mkRestrFrames.2 q.+1 (⇑ Hq) ε
+    (mkRestrFrames.2 r.+1 (⇑ (Hr ↕ ↑ Hq)) ω
+      (mkRestrFrames.2 s.+1 (⇑ (Hs ↕ ↑ (Hr ↕ ↑ Hq))) θ d)) =
+  (mkRestrFrames.2 s.+1 (⇑ (Hs ↕ (Hr ↕ Hq))) θ
+    (mkRestrFrames.2 r.+2 (⇑ (⇑ Hr ↕ ⇑ Hq)) ω
+      (mkRestrFrames.2 q.+3 (⇑ (⇑ (⇑ Hq))) ε d))).
+
+Definition mkCoh2LayerEndpointType {p k}
+  (depsCohs2: DepsCohs2 p.+1 k)
+  (extraDepsCohs2: DepsCohs2Extension p.+1 k depsCohs2)
+  (coh2Frames: mkCoh2FrameTypes (mkCohPaintings (depsCohs2; extraDepsCohs2)))
+  q (Hq: q <= k) r (Hr: r <= q) s (Hs: s <= r) (ε ω θ: arity)
+  (d: mkFrame (mkDepsRestr (depsCohs :=
+    toDepsCohs (mkCohFrames _ coh2Frames.1).1)).(1))
+  (l: mkLayer (mkDepsRestr (depsCohs :=
+    toDepsCohs (mkCohFrames _ coh2Frames.1).1)).(_restrFrames) d)
+  (coh2FrameEndpoint: mkCoh2FrameEndpointType depsCohs2
+    extraDepsCohs2 coh2Frames q Hq r Hr s Hs ε ω θ d): Type :=
+  let depsCohs := depsCohs2.(_depsCohs) in
+  let cohFrames1 := mkCohFrames depsCohs2.(_cohPaintings).1 depsCohs2.(_coh2Frames).1 in
+  let restrPaintings1 := mkRestrPaintings (depsCohs; depsCohs2.(_extraDepsCohs)) in
+  let cohFrames2 := mkCohFrames (mkCohPaintings (depsCohs2; extraDepsCohs2)).1 coh2Frames.1 in
+  let restrPaintings2 := mkRestrPaintings ((mkDepsCohs depsCohs2).(1);
+    (mkDepsCohs depsCohs2; mkExtraCohs extraDepsCohs2)) in
+  rew [mkLayer depsCohs.(_deps).(_restrFrames)] coh2FrameEndpoint in
+  mkRestrLayer depsCohs.(_restrPaintings) depsCohs.(_cohs) q Hq ε
+    (mkRestrFrame r.+1 (⇑ (Hr ↕ ↑ Hq)) ω
+      (mkRestrFrame s.+1 (⇑ (Hs ↕ ↑ (Hr ↕ ↑ Hq))) θ d))
+    (mkRestrLayer restrPaintings1 cohFrames1 r (Hr ↕ ↑ Hq) ω
+      (mkRestrFrame s.+1 (⇑ (Hs ↕ ↑ (Hr ↕ ↑ Hq))) θ d)
+      (mkRestrLayer restrPaintings2 cohFrames2 s (Hs ↕ ↑ (Hr ↕ ↑ Hq)) θ d l)) =
+  mkRestrLayer depsCohs.(_restrPaintings) depsCohs.(_cohs) s (Hs ↕ (Hr ↕ Hq)) θ
+    (mkRestrFrame r.+2 (⇑ (⇑ Hr ↕ ⇑ Hq)) ω
+      (mkRestrFrame q.+3 (⇑ (⇑ (⇑ Hq))) ε d))
+    (mkRestrLayer restrPaintings1 cohFrames1 r.+1 (⇑ Hr ↕ ⇑ Hq) ω
+      (mkRestrFrame q.+3 (⇑ (⇑ (⇑ Hq))) ε d)
+      (mkRestrLayer restrPaintings2 cohFrames2 q.+2 (⇑ (⇑ Hq)) ε d l)).
+
+Definition mkCoh2LayerType {p k}
+  (depsCohs2: DepsCohs2 p.+1 k)
+  (extraDepsCohs2: DepsCohs2Extension p.+1 k depsCohs2)
+  (coh2Frames: mkCoh2FrameTypes (mkCohPaintings (depsCohs2;extraDepsCohs2)))
+  q (Hq: q <= k) r (Hr: r <= q) s (Hs: s <= r) (ε ω θ: arity)
+  (d: mkFrame (mkDepsRestr (depsCohs :=
+    toDepsCohs (mkCohFrames _ coh2Frames.1).1)).(1))
+  (l: mkLayer (mkDepsRestr (depsCohs :=
+    toDepsCohs (mkCohFrames _ coh2Frames.1).1)).(_restrFrames) d): Type :=
+  let depsCohs := depsCohs2.(_depsCohs) in
+  let depsCohs' := toDepsCohs (mkCohFrames _ coh2Frames.1) in
+  rew [mkCoh2LayerEndpointType depsCohs2 extraDepsCohs2 coh2Frames q Hq r Hr s Hs ε ω θ d l]
+    coh2Frames.2 q.+1 (⇑ Hq) r.+1 (⇑ Hr) s.+1 (⇑ Hs) ε ω θ d in
+  (sigT_map_eq (Q := fun x => GDom (mkLayer _ x))
+    (mkRestrLayer depsCohs2.(_depsCohs).(_restrPaintings)
+      depsCohs2.(_depsCohs).(_cohs) q Hq ε)
+    (mkCohLayer (mkCohPaintings extraDepsCohs2).1
+      coh2Frames.2 r (Hr ↕ ↑ Hq) s Hs ω θ d l)
+  ⊙ (mkCohLayer depsCohs2.(_cohPaintings)
+      depsCohs2.(_coh2Frames).2 q Hq s (Hs ↕ Hr) ε θ
+      (mkRestrFrame r.+1 (⇑ (Hr ↕ ↑ Hq)) ω (d; l)).1
+      (mkRestrFrame r.+1 (⇑ (Hr ↕ ↑ Hq)) ω (d; l)).2
+  ⊙[fun x => GDom (mkLayer _ x)]
+    sigT_map_eq (Q := fun x => GDom (mkLayer _ x))
+      (mkRestrLayer depsCohs2.(_depsCohs).(_restrPaintings)
+        depsCohs2.(_depsCohs).(_cohs) s (Hs ↕ (Hr ↕ Hq)) θ)
+      (mkCohLayer (mkCohPaintings extraDepsCohs2).1 coh2Frames.2
+        q.+1 (⇑ Hq) r.+1 (⇑ Hr) ε ω d l))) =
+  mkCohLayer depsCohs2.(_cohPaintings)
+    depsCohs2.(_coh2Frames).2 q Hq r Hr ε ω
+    (mkRestrFrame s (↑ (↑ (Hs ↕ (Hr ↕ Hq)))) θ (d; l)).1
+    (mkRestrFrame s (↑ (↑ (Hs ↕ (Hr ↕ Hq)))) θ (d; l)).2
+  ⊙[fun x => GDom (mkLayer _ x)]
+    (sigT_map_eq (Q := fun x => GDom (mkLayer _ x))
+      (mkRestrLayer depsCohs2.(_depsCohs).(_restrPaintings)
+        depsCohs2.(_depsCohs).(_cohs) r (Hr ↕ Hq) ω)
+      (mkCohLayer (mkCohPaintings extraDepsCohs2).1
+        coh2Frames.2 q.+1 (⇑ Hq) s (↑ (Hs ↕ Hr)) ε θ d l)
+  ⊙ mkCohLayer depsCohs2.(_cohPaintings)
+      depsCohs2.(_coh2Frames).2 r (Hr ↕ Hq) s Hs ω θ
+      (mkRestrFrame q.+2 (⇑ (⇑ Hq)) ε (d; l)).1
+      (mkRestrFrame q.+2 (⇑ (⇑ Hq)) ε (d; l)).2).
+
+Definition mkCoh2Layer {p k}
+  (depsCohs2: DepsCohs2 p.+1 k)
+  (extraDepsCohs2: DepsCohs2Extension p.+1 k depsCohs2)
+  (coh2Frames: mkCoh2FrameTypes (mkCohPaintings (depsCohs2;extraDepsCohs2)))
+  q (Hq: q <= k) r (Hr: r <= q) s (Hs: s <= r) (ε ω θ: arity)
+  (d: mkFrame (mkDepsRestr (depsCohs :=
+    toDepsCohs (mkCohFrames _ coh2Frames.1).1)).(1))
+  (l: mkLayer (mkDepsRestr (depsCohs :=
+    toDepsCohs (mkCohFrames _ coh2Frames.1).1)).(_restrFrames) d):
+  mkCoh2LayerType depsCohs2 extraDepsCohs2 coh2Frames q Hq r Hr s Hs ε ω θ d l.
+Proof.
+  unfold mkCoh2LayerType.
+  admit.
+Admitted.
+
 Fixpoint mkCoh2Frames `{depsCohs2: DepsCohs2 p k}
   (extraDepsCohs2: DepsCohs2Extension p k depsCohs2):
   mkCoh2FrameTypes (mkCohPaintings extraDepsCohs2).
@@ -654,8 +757,7 @@ Proof.
       rewrite 4 eq_trans_eq_existT_curried.
       unshelve eapply eq_existT_curried_eq.
       * now exact (h.2 q.+1 (⇑ Hq) r.+1 (⇑ Hr) s.+1 (⇑ Hs) ε ω θ d).
-      * rewrite rew_map_eq_l.
-        admit.
-Admitted.
+      * now exact (mkCoh2Layer depsCohs2 extraDepsCohs2 h q Hq r Hr s Hs ε ω θ d l).
+Defined.
 
 End νGpd.
